fonction fields

examples/Sek/EChunkImpl.ml
@@ -3,68 +3,71 @@ open Capacity
 (** Type pour des buffers circulaires de capacité fixe K   TODO TRANSLATE ALL*)
 
 type 'a echunk = { (* TODO: remove prefixes *)
-  e_data : 'a array;
-  mutable e_front : int;
-  mutable e_size : int;
-  e_default : 'a }
+  data : 'a array;
+  mutable front : int;
+  mutable size : int;
+  default : 'a }
+
+let echunk_fields c =
+  c.data, c.front, c.size, c.default
 
 let echunk_default c =
-  c.e_default
+  c.default
 
 let echunk_dummy d = {
-  e_data = [||];
-  e_front = 0;
-  e_size = 0;
-  e_default = d
+  data = [||];
+  front = 0;
+  size = 0;
+  default = d
 }
 
 let echunk_create d = {
-  e_data = Array.make capacity d;
-  e_front = 0;
-  e_size = 0;
-  e_default = d
+  data = Array.make capacity d;
+  front = 0;
+  size = 0;
+  default = d
 }
 
 let echunk_is_empty c =
-  c.e_size = 0
+  c.size = 0
 
 let echunk_is_full c =
-  c.e_size = capacity
+  c.size = capacity
 
 let echunk_peek_back c =
-  let back = wrap_up (c.e_front + c.e_size - 1) in
-  c.e_data.(back)
+  let back = wrap_up (c.front + c.size - 1) in
+  c.data.(back)
 
 let echunk_pop_back c =
   let x = echunk_peek_back c in
-  let new_size = c.e_size - 1 in
-  c.e_size <- new_size;
-  let i = wrap_up (c.e_front + new_size) in
-  c.e_data.(i) <- c.e_default;
+  let new_size = c.size - 1 in
+  c.size <- new_size;
+  let i = wrap_up (c.front + new_size) in
+  c.data.(i) <- c.default;
   x
 
 let echunk_push_back c x =
-  let old_size = c.e_size in
-  c.e_size <- old_size + 1;
-  let i = wrap_up (c.e_front + old_size) in
-  c.e_data.(i) <- x
+  let old_size = c.size in
+  c.size <- old_size + 1;
+  let i = wrap_up (c.front + old_size) in
+  c.data.(i) <- x
 
 let echunk_peek_front c =
-  c.e_data.(c.e_front)
+  c.data.(c.front)
 
 let echunk_pop_front c =
   let x = echunk_peek_front c in
-  let old_front = c.e_front in
-  c.e_size <- c.e_size - 1;
-  c.e_front <- wrap_up (old_front + 1);
-  c.e_data.(old_front) <- c.e_default;
+  let old_front = c.front in
+  c.size <- c.size - 1;
+  c.front <- wrap_up (old_front + 1);
+  c.data.(old_front) <- c.default;
   x
 
 let echunk_push_front c x =
-  let new_front = wrap_down (c.e_front - 1) in
-  c.e_size <- c.e_size + 1;
-  c.e_front <- new_front;
-  c.e_data.(new_front) <- x
+  let new_front = wrap_down (c.front - 1) in
+  c.size <- c.size + 1;
+  c.front <- new_front;
+  c.data.(new_front) <- x
 
 (* let echunk_get c i =
   c.data.(i)
